src/Bedrock/Field/Translation/Proofs/Cmd.v
@@ -5,11 +5,13 @@ Require Import Coq.Strings.String.
 Require Import bedrock2.ProgramLogic.
 Require Import bedrock2.Map.Separation.
 Require Import bedrock2.Map.SeparationLogic.
+Require Import bedrock2.WeakestPrecondition.
 Require Import bedrock2.WeakestPreconditionProperties.
 Require Import coqutil.Map.Interface.
 Require Import coqutil.Word.Interface.
 Require Import coqutil.Datatypes.List.
 Require Import coqutil.Datatypes.PropSet.
+Require Import coqutil.Z.PushPullMod.
 Require Import Crypto.Bedrock.Field.Common.Types.
 Require Import Crypto.Bedrock.Field.Common.Tactics.
 Require Import Crypto.Bedrock.Field.Common.Util.
@@ -33,9 +35,8 @@ Import Wf.Compilers.expr.
 Import Types.Notations.
 
 Section Cmd.
-  Context 
+  Context
     {width BW word mem locals env ext_spec varname_gen add_carryx sub_borrowx error}
-    {add_carryx_funcname sub_borrowx_funcname : string}
    `{parameters_sentinel : @parameters width BW word mem locals env ext_spec varname_gen add_carryx sub_borrowx error}.
   Context {ok : ok}.
 
@@ -97,6 +98,19 @@ Section Cmd.
                                 (expr.Ident (ident.Literal (t:=base.type.Z) s)))
                       x) y)) f)
   .
+
+  Local Instance spec_of_add_carryx : spec_of add_carryx :=
+    fnspec! add_carryx x y carry ~> sum carry_out,
+    { (* The required upper bound on `carry` isn't necessary for the
+         current `add_with_carry` to support the `ensures` clause, but
+         it does formalize an expected condition that future
+         implementations should be free to leverage. *)
+      requires t m := word.unsigned carry < 2;
+      ensures T M :=
+        M = m /\ T = t /\
+        word.unsigned sum + 2^width * word.unsigned carry_out =
+        word.unsigned x + word.unsigned carry + word.unsigned y
+    }.
 
   Lemma assign_list_correct :
     forall (rhs : base_rtype base_listZ)
@@ -319,9 +333,7 @@ Section Cmd.
         G nextn :
     valid_expr true e1 ->
     wf3 G e1 e2 e3 ->
-    translate_cmd (add_carryx_funcname:=add_carryx_funcname)
-                  (sub_borrowx_funcname:=sub_borrowx_funcname)
-                  e3 nextn = assign nextn (translate_expr true e3).
+    translate_cmd e3 nextn = assign nextn (translate_expr true e3).
   Proof.
     inversion 1; cleanup_wf; try reflexivity; intros.
     all: repeat first [ reflexivity
@@ -329,6 +341,230 @@ Section Cmd.
                         | [ H : wf3 _ ?x _ _ |- _ ]
                           => assert_fails is_var x; inversion H; clear H; cleanup_wf
                         end ].
+  Qed.
+
+  Lemma max_range_good : range_good (width:=width) (max_range (width:=width)) = true.
+  Proof.
+    cbv [range_good].
+    destruct (ZRange.reflect_zrange_eq (max_range (width:=width))
+                                       (max_range (width:=width))); congruence.
+  Qed.
+
+  Ltac invert_wf3_until_exposed :=
+    repeat match goal with
+           | _ => progress cleanup_wf
+           | H : wf3 _ ?x ?y _ |- _ =>
+             progress match x with
+                      | expr.App _ _ =>
+                        progress match y with
+                                 | expr.App _ _ => idtac (* already inverted *)
+                                 | _ => inversion H; clear H
+                                 end
+                        | expr.Ident _ =>
+                          progress match y with
+                                   | expr.Ident _ _ => idtac (* already inverted *)
+                                   | _ => inversion H; clear H
+                                   end
+                        | expr.Var _ =>
+                          progress match y with
+                                   | expr.Var _ _ => idtac (* already inverted *)
+                                   | _ => inversion H; clear H
+                                   end
+                      end
+           end.
+
+  Lemma valid_expr_not_special3 {t}
+        (e1 : @API.expr (fun _ => unit) t)
+        (e2 : @API.expr API.interp_type t)
+        (e3 : @API.expr ltype t) G :
+    valid_expr false e1 ->
+    wf3 G e1 e2 e3 ->
+    forall nextn, translate_if_special3 e3 nextn = None.
+  Proof.
+    induction 1; intros; invert_wf3_until_exposed; reflexivity.
+  Qed.
+
+
+  Lemma invert_App_Z_cast_Some {var} (x : @API.expr var type_Z) r :
+    invert_expr.invert_App_Z_cast
+      (expr.App (expr.App (expr.Ident ident.Z_cast)
+                          (expr.Ident (ident.Literal r)))
+                x) = Some (r, x).
+  Proof. reflexivity. Qed.
+
+  Lemma invert_App_Z_cast2_Some {var} (x : @API.expr var type_ZZ) r1 r2 :
+    invert_expr.invert_App_Z_cast2
+      (expr.App (expr.App (expr.Ident ident.Z_cast2)
+                          (expr.App (expr.App (expr.Ident ident.pair)
+                                              (expr.Ident (ident.Literal r1)))
+                                              (expr.Ident (ident.Literal r2))))
+                x) = Some (r1, r2, x).
+  Proof. reflexivity. Qed.
+
+  Lemma valid_expr_not_special_function {t}
+        (e1 : @API.expr (fun _ => unit) t)
+        (e2 : @API.expr API.interp_type t)
+        (e3 : @API.expr ltype t) G :
+    valid_expr true e1 ->
+    wf3 G e1 e2 e3 ->
+    forall nextn, translate_if_special_function e3 nextn = None.
+  Proof.
+    induction 1; intros; invert_wf3_until_exposed;
+      try reflexivity; cbv [translate_if_special_function invert_expr.invert_App_cast].
+    { rewrite invert_App_Z_cast_Some.
+      cbn. erewrite valid_expr_not_special3 by eauto. break_innermost_match; reflexivity. }
+    { rewrite invert_App_Z_cast2_Some.
+      cbn. erewrite valid_expr_not_special3 by eauto. break_innermost_match; reflexivity. }
+  Qed.
+
+  (* Convenience lemma for add_with_get_carry case. *)
+  Lemma add_get_carry_full_equiv (x y sum carry_out : @word.rep width word) r1 r2:
+    word.unsigned sum + 2^width * word.unsigned carry_out
+    = word.unsigned x + word.unsigned y ->
+    range_good (width:=width) r1 = true -> range_good (width:=width) r2 = true ->
+    PreExtra.ident.cast2
+      (r1, r2)
+      (Definitions.Z.add_get_carry_full
+         (2 ^ width) (word.unsigned x) (word.unsigned y))
+    = (word.unsigned sum, word.unsigned carry_out).
+  Proof.
+    pose proof word.width_pos. intro Heq. intros.
+    pose proof (Properties.word.unsigned_range x).
+    pose proof (Properties.word.unsigned_range y).
+    pose proof (Properties.word.unsigned_range sum).
+    pose proof (Properties.word.unsigned_range carry_out).
+    repeat lazymatch goal with
+           | H : range_good _ = true |- _ => apply range_good_eq in H; subst
+           end.
+    cbv [Definitions.Z.add_get_carry_full
+           Definitions.Z.add_with_get_carry
+           Definitions.Z.add_with_carry
+           Definitions.Z.add_get_carry
+           Definitions.Z.get_carry
+           PreExtra.ident.cast2
+           Rewriter.Util.LetIn.Let_In
+        ].
+    cbn [fst snd]. rewrite Z.log2_pow2, Z.eqb_refl by lia.
+    cbn [fst snd]. rewrite Z.add_0_l.
+    rewrite !CastLemmas.ident.cast_in_bounds by (apply is_bounded_by_bool_max_range; Z.div_mod_to_equations; nia).
+    rewrite <-Heq. apply f_equal2.
+    { Z.push_mod. rewrite Z.mod_same by lia. Z.push_pull_mod.
+      rewrite Z.mod_small; lia. }
+    { Z.div_mod_to_equations; nia. }
+  Qed.
+
+  (* Convenience lemma for add_with_get_carry case. *)
+  Lemma add_with_get_carry_full_equiv (x y sum carry_in carry_out : @word.rep width word) r1 r2:
+    word.unsigned sum + 2^width * word.unsigned carry_out
+    = word.unsigned carry_in + word.unsigned x + word.unsigned y ->
+    range_good (width:=width) r1 = true -> range_good (width:=width) r2 = true ->
+    PreExtra.ident.cast2
+      (r1, r2)
+      (Definitions.Z.add_with_get_carry_full
+         (2 ^ width) (word.unsigned carry_in) (word.unsigned x) (word.unsigned y))
+    = (word.unsigned sum, word.unsigned carry_out).
+  Proof.
+    pose proof word.width_pos. intro Heq. intros.
+    pose proof (Properties.word.unsigned_range x).
+    pose proof (Properties.word.unsigned_range y).
+    pose proof (Properties.word.unsigned_range carry_in).
+    pose proof (Properties.word.unsigned_range sum).
+    pose proof (Properties.word.unsigned_range carry_out).
+    repeat lazymatch goal with
+           | H : range_good _ = true |- _ => apply range_good_eq in H; subst
+           end.
+    cbv [Definitions.Z.add_with_get_carry_full
+           Definitions.Z.add_with_get_carry
+           Definitions.Z.add_with_carry
+           Definitions.Z.get_carry
+           PreExtra.ident.cast2
+           Rewriter.Util.LetIn.Let_In
+        ].
+    cbn [fst snd]. rewrite Z.log2_pow2, Z.eqb_refl by lia.
+    cbn [fst snd].
+    rewrite !CastLemmas.ident.cast_in_bounds by (apply is_bounded_by_bool_max_range; Z.div_mod_to_equations; nia).
+    rewrite <-Heq. apply f_equal2.
+    { Z.push_mod. rewrite Z.mod_same by lia. Z.push_pull_mod.
+      rewrite Z.mod_small; lia. }
+    { Z.div_mod_to_equations; nia. }
+  Qed.
+
+  (* TODO: move to equivalence *)
+  Lemma locally_equiv_pair l w1 w2 n1 n2 z1 z2 :
+    n1 <> n2 ->
+    word.unsigned w1 = z1 ->
+    word.unsigned w2 = z2 ->
+    locally_equivalent (t:=type_ZZ) (z1, z2)
+                       (Syntax.expr.var n1, Syntax.expr.var n2)
+                       (map.put (map.put l n1 w1) n2 w2).
+  Proof.
+    intros; repeat eexists; cbn [fst snd];
+      repeat lazymatch goal with
+               | |- context [map.putmany map.empty _] =>
+                 rewrite Properties.map.putmany_empty_l
+               | |- context [map.disjoint map.empty _] =>
+                 apply Properties.map.disjoint_empty_l
+               | H : word.unsigned _ = ?z |- word.unsigned _ = ?z => exact H
+               | |- context [map.get (map.put _ ?k _) ?k] =>
+                 rewrite map.get_put_same
+               | |- context [map.get (map.put _ _ _) _] =>
+                 rewrite map.get_put_diff by congruence
+               | _ => reflexivity
+             end.
+  Qed.
+
+  Lemma invert_Literal_Some {var t} (x : Compilers.base_interp t) :
+    invert_expr.invert_Literal (var:=var) (expr.Ident (ident.Literal x)) = Some x.
+  Proof. reflexivity. Qed.
+
+  Lemma invert_AppIdent3_Some {Q R S a b c d var} (i : ident (a -> b -> c -> d))
+        (x : expr a) (y : expr b) (z : expr c)
+        (f1 : forall t x, Q t)
+        (f2 : forall t x, R t)
+        (f3 : forall t x, S t) :
+    invert_AppIdent3_cps (var:=var) (expr.App (expr.App (expr.App (expr.Ident i) x) y) z) f1 f2 f3
+    = Some (existT _ (a, b, c) (i, f1 _ x, f2 _ y, f3 _ z)).
+  Proof. reflexivity. Qed.
+
+  Lemma translate_add_get_carry nextn (x y : API.expr type_Z) r1 r2 :
+    range_good (width:=width) r1 = true ->
+    range_good (width:=width) r2 = true ->
+    let sum := varname_gen nextn in
+    let carry := varname_gen (S nextn) in
+    translate_if_special_function
+      (expr.App
+         (expr.App (expr.Ident ident.Z_cast2)
+                   (expr.App
+                      (expr.App
+                         (expr.Ident ident.pair)
+                         (expr.Ident (ident.Literal (t:=base.type.zrange) r1)))
+                      (expr.Ident (ident.Literal (t:=base.type.zrange) r2))))
+         (expr.App
+            (expr.App
+               (expr.App (expr.Ident ident.Z_add_get_carry)
+                         (expr.Ident (ident.Literal (t:=base.type.Z) (2 ^ width))))
+               x) y)) nextn
+    = Some (2%nat, (sum,carry), Syntax.cmd.call [sum;carry] add_carryx [(translate_expr true x); (translate_expr true y); Syntax.expr.literal 0]).
+  Proof.
+    cbv [translate_if_special_function]; intros.
+    repeat lazymatch goal with H : range_good ?r = true |- _ => apply range_good_eq in H; subst end.
+    cbn [invert_expr.invert_App_cast
+           invert_expr.invert_App_Z_cast2
+           invert_expr.invert_App invert_expr.invert_App_cps].
+    lazymatch goal with
+      |- context [invert_expr.invert_Z_cast2 ?x] =>
+      replace (invert_expr.invert_Z_cast2 x) with
+        (Some (max_range (width:=width), max_range (width:=width)))
+        by reflexivity
+    end.
+    cbn [Crypto.Util.Option.bind fst snd range_type_good range_base_good].
+    rewrite !max_range_good. cbn [andb].
+    cbv [translate_if_special3]. rewrite invert_AppIdent3_Some.
+    cbn [Crypto.Util.Option.bind fst snd].
+    cbv [translate_ident_special3].
+    cbn [type.domain]. rewrite invert_Literal_Some.
+    cbn [Crypto.Util.Option.bind fst snd].
+    rewrite Z.eqb_refl. reflexivity.
   Qed.
 
   Local Ltac simplify :=
@@ -410,12 +646,12 @@ Section Cmd.
     forall functions
            (locals : locals)
            (nextn : nat),
+      (* specifications of bedrock2 functions we might call *)
+      spec_of_add_carryx functions ->
       (* ret := fiat-crypto interpretation of e2 *)
       let ret1 : API.interp_type t := API.interp e2 in
       (* out := translation output for e3 *)
-      let out := translate_cmd (add_carryx_funcname:=add_carryx_funcname)
-                               (sub_borrowx_funcname:=sub_borrowx_funcname)
-                               e3 nextn in
+      let out := translate_cmd e3 nextn in
       let nvars := fst (fst out) in
       let ret2 := rtype_of_ltype _ (snd (fst out)) in
       let body := snd out in
@@ -427,8 +663,7 @@ Section Cmd.
       (forall n nvars,
           (nextn <= n)%nat ->
           map.undef_on locals (used_varnames(varname_gen:=varname_gen) n nvars)) ->
-      forall tr
-             (mem : mem),
+      forall tr (mem : mem),
         (* contexts are equivalent; for every variable in the context list G,
              the fiat-crypto and bedrock2 results match *)
         context_equiv G locals ->
@@ -468,10 +703,10 @@ Section Cmd.
 
     (* simplify goals *)
     all:repeat match goal with
-               | H : range_good ?r = true |- _ => rewrite range_good_eq in H; subst
                | _ => progress (intros; cleanup)
                | _ => progress cbv [Rewriter.Util.LetIn.Let_In] in *
                | _ => erewrite translate_cmd_valid_expr by eauto
+               | _ => erewrite valid_expr_not_special_function by eauto
                | _ => progress cbn [translate_cmd expr.interp type.app_curried
                                                   WeakestPrecondition.cmd
                                                   WeakestPrecondition.cmd_body] in *
@@ -483,7 +718,6 @@ Section Cmd.
                end.
 
     { (* let-in (product of base types) *)
-      admit. (*
       eapply Proper_cmd; [ eapply Proper_call | repeat intro | ].
       2: {
         eapply IHe1_valid; clear IHe1_valid;
@@ -499,10 +733,7 @@ Section Cmd.
         apply used_varnames_disjoint; lia. }
       { simplify; subst; eauto; only_differ_ok.
         etransitivity; [ eassumption | ].
-        apply used_varnames_shift. } *) }
-    { (* let-in (base type) *)
-      admit.
-      (*
+        apply used_varnames_shift. } }
       eapply Proper_cmd; [ eapply Proper_call | repeat intro | ].
       2: {
         eapply IHe1_valid; clear IHe1_valid;
@@ -518,7 +749,7 @@ Section Cmd.
         apply used_varnames_disjoint; lia. }
       { simplify; subst; eauto; only_differ_ok.
         etransitivity; [ eassumption | ].
-        apply used_varnames_shift. } } *) }
+        apply used_varnames_shift. }
     { (* cons *)
       eapply Proper_cmd; [ eapply Proper_call | repeat intro | ].
       2: {
@@ -567,67 +798,90 @@ Section Cmd.
       match goal with H : PropSet.sameset _ _ |- _ =>
                       rewrite H end; reflexivity. }
     { (* add_get_carry *)
+      rewrite translate_add_get_carry by auto. cbn [fst snd].
+      cbn [WeakestPrecondition.cmd WeakestPrecondition.cmd_body].
+      repeat lazymatch goal with
+             | H : valid_expr _ ?e |- _ =>
+               lazymatch goal with
+               | Hwf : wf3 ?G e ?e2 ?e3 |- _ =>
+                 let Htr := fresh in
+                 pose proof translate_expr_correct e e2 e3 ltac:(eassumption) G _ Hwf ltac:(eassumption) as Htr;
+                   destruct Htr; sepsimpl
+               end;
+                 clear H
+             end.
+      eexists; split; [ | ].
+      { (* Argument expressions. *)
+        repeat lazymatch goal with
+               | |- dexprs _ _ (_ :: _) _ => apply dexprs_cons_iff; split
+               | H : dexpr map.empty ?l ?x _ |- WeakestPrecondition.expr ?m ?l ?x _ =>
+                 apply expr_empty; apply H
+               | _ => reflexivity
+               end. }
+      straightline_call; [ rewrite Properties.word.unsigned_of_Z_0; lia | ].
+      sepsimpl; subst; cleanup.
+      eexists; split; [ reflexivity | ].
       eapply Proper_cmd; [ eapply Proper_call | repeat intro | ].
       2:{
+        eapply IHe1_valid; clear IHe1_valid;
+        repeat match goal with
+               | _ => progress (intros; cleanup)
+               | H : forall v1 v2 v3, wf3 _ (?f v1) _ _ |- wf3 _ (?f tt) _ _ => solve [apply (H tt)]
+               | H : ?P |- ?P => exact H
+               end; [ | | ].
+        { (* context varname_set *)
+          new_context_ok.
+          lazymatch goal with
+          | H : rep.varname_set _ _ \/ rep.varname_set _ _ |- _ =>
+            cbn  in H; destruct H as [H | H]; apply varname_gen_unique in H; lia
+          end. }
+        { (* undef on *)
+          repeat lazymatch goal with
+                 | |- map.undef_on (map.put _ _ _) _ => apply put_undef_on
+                 | H : forall n nvars, _ -> map.undef_on ?l (used_varnames n nvars)
+                                  |- map.undef_on ?l (used_varnames _ _) =>
+                   apply H; lia
+                 | |- ~ used_varnames _ _ _ => rewrite used_varnames_iff; intro; simplify
+                 | H : varname_gen _ = varname_gen _ |- _ => apply varname_gen_unique in H; lia
+                 end. }
+        { (* context equivalent *)
+          apply Forall_cons;
+            [ apply locally_equiv_pair; eauto; rewrite varname_gen_unique; lia | ].
+          eapply equivalent_not_in_context_forall; eauto;
+            repeat lazymatch goal with
+                   | |- map.only_differ (map.put _ _ _) _ _ =>
+                     eapply only_differ_trans; [ | solve [apply only_differ_put] ]
+                   | |- map.only_differ ?m _ ?m => solve [apply only_differ_empty]
+                   | |- map.only_differ _ _ (map.put _ _ _) =>
+                     apply only_differ_sym
+                   | |- disjoint (union _ _) _ =>
+                     apply disjoint_union_l_iff; split
+                   | |- disjoint empty_set _ =>
+                     solve [apply disjoint_empty_l]
+                   | |- disjoint (singleton_set _) _ =>
+                     symmetry; apply disjoint_singleton_r_iff
+                   | _ => solve [eauto with lia]
+                   end. } }
+      clear IHe1_valid.
+      simplify; subst; eauto; [ | | ].
+      { (* varnames subset *)
+        rewrite <-used_varnames_shift; eauto. }
+      { (* only_differ *)
+        only_differ_ok.
+        eauto using only_differ_succ, only_differ_zero. }
+      { (* equivalence of output holds *)
         lazymatch goal with
-          |- context [translate_if_special_function ?x ?n] =>
-          remember (translate_if_special_function (add_carryx_funcname:=add_carryx_funcname)
-                                              (sub_borrowx_funcname:=sub_borrowx_funcname)
-                                              x n) as X eqn:HX
+        | H : equivalent_base ?x1 ?y ?a ?l ?m |- equivalent_base ?x2 ?y ?a ?l ?m =>
+          replace x2 with x1; [ exact H | ]
         end.
-        cbv [translate_if_special_function] in HX.
-        cbv [invert_expr.invert_App_cast invert_expr.invert_App_Z_cast2 invert_expr.invert_App invert_expr.invert_App_cps] in HX.
-        lazymatch type of HX with context [invert_expr.invert_Z_cast2 ?x] => pose x as z end.
-        Search range_good.
-        Print range_good.
-        vm_compute in z.
-        cbn in X.
-        cbv [
-            translate_if_special_function
-              invert_expr.invert_App_cast
-              invert_expr.invert_App_Z_cast
-              invert_expr.invert_App_Z_cast2
-              invert_expr.invert_Z_cast2
-              invert_expr.invert_App
-              invert_expr.invert_Ident
-              invert_expr.invert_AppIdent
-              invert_expr.invert_AppIdent_cps
-              invert_expr.invert_AppIdent2_cps
-              invert_expr.invert_App_cps
-              invert_expr.invert_App2_cps
-              invert_expr.invert_Literal
-              invert_expr.invert_pair
-              invert_expr.invert_pair_cps
-              invert_expr.is_pair
-              invert_expr.reflect_smart_Literal
-              Option.bind
-              Crypto.Util.Option.bind
-          ] in X.
-        clear IHe1_valid.
-        cbv [Option.bind Crypto.Util.Option.bind].
-        eapply IHe1_valid with (G:=G); clear IHe1_valid;
-        repeat match goal with
-               | _ => progress (intros; cleanup)
-               | H : _ |- _ => solve [apply H]
-               | _ => solve [new_context_ok]
-               | _ => congruence
-               end; [ ].
-        eapply only_differ_disjoint_undef_on; eauto with lia; [ ].
-        match goal with H : PropSet.sameset _ _ |- _ => rewrite H end.
-        apply used_varnames_disjoint. lia. }
-        cbn.
-        cbn [translate_expr].
-        repeat match goal with
-               | _ => progress (intros; cleanup)
-               | H : _ |- _ => solve [apply H]
-               | _ => solve [new_context_ok]
-               | _ => congruence
-               end; [ ].
-        eapply only_differ_disjoint_undef_on; eauto with lia; [ ].
-        match goal with H : PropSet.sameset _ _ |- _ =>
-                        rewrite H end.
-        apply used_varnames_disjoint; lia. 
-        
-      }
+        lazymatch goal with
+          | H : context [word.unsigned (word.of_Z 0)] |- _ =>
+            rewrite Properties.word.unsigned_of_Z_0 in H
+        end.
+        repeat lazymatch goal with
+               | H : word.unsigned _ = expr.interp ?iinterp ?x |- context [expr.interp ?iinterp ?x] =>
+                 rewrite <-H
+               end.
+        erewrite add_get_carry_full_equiv; eauto with lia. } }
   Qed.
 End Cmd.
